\documentclass[../main.tex]{subfiles}
\begin{document}
\chapter{The M\"obius Group}
\section{Introduction and Definitions}
This chapter is all about a group called the \textit{M\"obius Group}.
It is \textit{almost} a group of bijections of $\C$ \textbf{but} we need to add a formal ``point at infinity''.
\subsection{Riemann Sphere and M\"obius Transforms}
\begin{definition}[Riemann Sphere]
  The \textit{Riemann sphere}, $\Cinf$, is defined to be:
  \[
    \Cinf = \C \cup \{\infty\}
  \]
\end{definition}
We define $\pi(z)$ to be the \textit{stereographic projection} of $z \in \C$ onto $S^2$ (The unit sphere).
If we draw a line through $z$ and the north pole, this line will intersect the sphere exactly once, this is $\pi(z)$.
The stereographic projection identified $\C$ with all the points of the sphere except the north pole, which we define to be $\infty$.
\begin{definition}[M\"obius Transform]
  Let $a, b, c, d \in \C$ such that $ad - bc \neq 0$.
  The \textit{m\"obius transform}, $\mu: \Cinf \to \Cinf$ is defined as:

  For $c \neq 0$:
  \[
    z \mapsto \begin{cases}
    \frac{az + b}{cz + d} & \text{if $z \in \C \setminus \{-\frac{d}{c}\}$} \\
    \infty & \text{if $z = -\frac{d}{c}$} \\
    \frac{a}{c} & \text{if $z = \infty$}
    \end{cases}
  \]
  For $c = 0$:
  \[
    z \mapsto \begin{cases}
    \frac{az + b}{d} & \text{if $z \in \C$} \\
    \infty & \text{if $z = \infty$}
    \end{cases}
  \]
\end{definition}
For brevity, we usually just write:
\[
  ``\mu(z) = \frac{az + b}{cz + b} \text{, interpreting the cases of $0$ and $\infty$ appropriately''}
\]
\section{M\"obius Group}
\begin{definition}[M\"obius Group]
  The set $\mob$:
  \[
    \mob = \{f: \Cinf \to \Cinf: f \text{ is a M\"obius transform}\}
  \]
  together with composition is the \textit{M\"obius Group}.
\end{definition}

\begin{proposition}
  The composition of two M\"obius transforms is also a M\"obius transform.
  \label{mobComposition}
\end{proposition}
\begin{proof}
  If we take:
  \[
    \mu_1(z) = \frac{a_1 z + b_1}{c_1 z + d_1},\
    \mu_2(z) = \frac{a_2 z + b_2}{c_2 z + d_2}
  \]
  Then we see that $\mu_1 \circ \mu_2$ is:
  \begin{align*}
    \mu_1 \circ \mu_2 (z) &= \frac{a_1\mu_2(z) + b_1}{c_1\mu_2(z) + d_1} \\
                          &= \frac{a_1\left(\frac{a_2 z + b_2}{c_2 z + d_2}\right) + b_1}{c_1\left(\frac{a_2 z + b_2}{c_2 z + d_2}\right) + d_1} \\
                          &= \frac{a_1(a_2 z + b_2) + b_1(c_2 z + d_2)}{c_1(a_2 z + b_2) + d_1(c_2 z + d_2)} \\
                          &= \frac{\overbrace{(a_1 a_2 + b_1 c_2)}^{a'}z + \overbrace{(a_1 b_2 + b_1 d_2)}^{b'}}{\underbrace{(c_1 a_2 + d_1 c_2)}_{c'}z + \underbrace{(c_1 b_2 + d_1 d_2)}_{d'}}
  \end{align*}
  So $\mu_1 \circ \mu_2$ is in the correct form.
  We now need to check that it satisfies $a'd' - b'c' \neq 0$:
  \begin{align*}
    a'd' - b'c' &= (a_1 a_2 + b_1 c_2)(c_1 b_2 + d_1 d_2) - (a_1 b_2 + b_1 d_2)(c_1 a_2 + d_1 c_2) \\
                &= \cancel{a_1 a_2 c_1 b_2} + b_1 b_2 c_1 c_2 + a_1 a_2 d_1 d_2 + \cancel{d_1 d_2 b_1 c_2}\\
                &\quad- \cancel{a_1 a_2 c_1 b_2} - b_1 c_1 a_2 d_2 - a_1 d_1 b_2 c_2 - \cancel{d_1 d_2 b_1 c_2} \\
                &= a_2 d_2(a_1 d_1 - b_1 c_1) - b_2 c_2(a_2 d_2 - b_2 c_2) \\
                &= (a_1 d_1 - b_1 c_1)(a_2 d_2 - b_2 c_2)
  \end{align*}
  Since $\mu_1$ and $\mu_2$ are M\"obius transforms, $a_1 d_1 - b_1 c_2 \neq 0$ and $a_2 d_2 - b_2 c_2 \neq 0$.
  Therefore $a'd' - b'c' \neq 0$, so $\mu_1 \circ \mu_2 \in \mob$.
\end{proof}
\begin{remark}
  $a', b', c', d'$ described above are the entries obtained when multiplying the following two matrices:
  \[
    \begin{pmatrix}
    a_1 & b_1 \\
    c_1 & d_1 \\
    \end{pmatrix}
    \begin{pmatrix}
    a_2 & b_2 \\
    c_2 & d_2 \\
    \end{pmatrix} =
    \begin{pmatrix}
    a_1a_2 + b_1c_2 & a_1b_2 + b_1d_2 \\
    c_1a_2 + d_1c_2 & c_1b_2 + d_1d_2 \\
    \end{pmatrix}
  \]
\end{remark}
\begin{theorem}[M\"obius Group]
  $(\mob, \circ, \id)$ is a group.
\end{theorem}
\begin{proof}
  \begin{itemize}
    \item \textbf{Associativity -} Composition of functions is associative, see \cref{assocLemma}.
    \item \textbf{Identity -}
      \[
        \id: z \mapsto z = \frac{1\cdot z + 0}{0 \cdot z + 1} \in \mob
      \]
    \item \textbf{Inverses -} Let:
      \[
        \mu: z \mapsto \frac{az + b}{cz + d},\ \nu: z \mapsto \frac{dz - b}{-cz + a}
      \]
      Then by \cref{mobComposition}:
      \[
        \mu \circ \nu = \left(\frac{ad - bc}{ad - bc}\right)z =z
      \]
      So $\mu^{-1} = \nu \in \mob$.
    \item \textbf{Closure -} See \cref{mobComposition}.
  \end{itemize}
\end{proof}
\section{Fixed Points}
One important way to study M\"obius transforms is via their fixed points.
\begin{definition}
  Suppose $f: X \to X$ is a permutation.
  Any $x \in X$ such that $f(x) = x$ is called a \textit{fixed point} of $f$.
\end{definition}
\begin{remark}[Notation]
  We denote the set of fixed points of a function $f$ as $\Fix(f)$.
\end{remark}
\begin{lemma}[3-point Lemma for $\mob$]
  If $\mu \in \mob$ fixes three distinct points $w_1, w_2, w_3 \in \Cinf$, then $\mu = \id$.
  \label{threePointMob}
\end{lemma}
\begin{proof}
  Let $\mu(z) = \frac{az + b}{cz + d}$.
  A fixed point $w_i$ satisfies the equation:
  \[
    w_i = \frac{aw_i + b}{cw_i + d}
  \]
  \begin{proofcases}
    \begin{case}{One $w_i$ is infinite}
      WLOG suppose $w_1 = \infty$, then $c = 0$ so $w_2$ and $w_3$ satisfy:
      \[
        w_i = \frac{aw_i + b}{d} \iff (a-d)w_i + b = 0
      \]
      This is a linear equation with at least 2 distinct roots so must be trivial, that is, $a = d$ and $b = 0$.
      So $\mu(z) = \frac{az}{d} = z = \id$.
    \end{case}
    \begin{case}{$w_i \neq \infty$}
      Now suppose every $w_i \neq \infty$.
      \begin{align*}
        w_i &= \frac{aw_i + b}{cw_i + d} \\
        cw^{2}_{i} + dw_i &= aw_i + b \\
        cw^{2}_{i} + (d - a)w_i - b &= 0
      \end{align*}
      This is a quadratic with at least 3 roots so must be trivial, that is, $b = c = 0$ and $a = d$.
      So again $\mu(z) = \id$.
    \end{case}
  \end{proofcases}
\end{proof}
\begin{proposition}
  Every $\mu \in \mob$ has at least one fixed point in $\Cinf$.
\end{proposition}
\begin{proof}
  \begin{proofcases}
    \begin{case}{$c = 0$}
      Then, by definition, $\mu(\infty) = \infty$ so $\infty \in \Fix(\mu)$.
    \end{case}
    \begin{case}{$c \neq 0$}
      A fixed point of $\mu$ satisfies:
      \[
        \mu(z) = \frac{az + b}{cz + d} = z \\
        \iff az + b = cz^2 + dz \\
        \iff cz^2 + (d - a)z - b = 0
      \]
      Since $c \neq 0$, this is a quadratic so has either one repeated or two distinct complex roots.
      Note that $z = -\frac{d}{c}$ cannot be a root otherwise we would have:
      \begin{align*}
        c\left(-\frac{d}{c}\right)^2 + \left(-\frac{d}{c}\right)(d-a) - b &= 0 \\
        \frac{d^2}{c} - \frac{d^2}{c} + \frac{ad}{c} - b &= 0 \\
        \frac{ad}{c} - b &= 0 \\
        ad - bc &= 0
      \end{align*}
      So we must have at least one $z$ satisfying $\mu(z) = z$.
    \end{case}
    In both cases, $\mu$ fixes at least one point.
  \end{proofcases}
\end{proof}
\begin{example}
  \begin{enumerate}
    \item If $\mu(z) = z + 1$, then $\Fix(\mu) = \{\infty\}$.
    \item If $\mu(z) = 2z$, then $\Fix(\mu) = \{0, \infty\}$.
  \end{enumerate}
\end{example}
\begin{lemma}[Triple Transitivity]
  For any triples of distinct points $z_1, z_2, z_3 \in \Cinf$ and $w_1, w_2, w_3 \in \Cinf$ there exists a $\mu \in \mob$ such that $\mu(z_i) = w_i$ for $i = 1, 2, 3$.
  \label{tripleTransitivity}
\end{lemma}
\begin{proof}
  Let
  \[
    \alpha(z) = \left(\frac{z - z_1}{z - z_3}\right) \left(\frac{z_2 - z_3}{z_2 - z_1}\right)
  \]
  \begin{remark}[Note]
    If one of $z_i$ is infinite, then we can modify $\alpha$ to be:
    \[
      z_1 = \infty \to \frac{z_2 - z_3}{z - z_3},\ z_2 = \infty \to \frac{z - z_1}{z - z_3}, z_3 = \infty \to \frac{z - z_1}{z_2 - z_1}
    \]
    and the following still holds true.
  \end{remark}
  We can now see that:
  \[
    \alpha: z_1 \mapsto 0,\ z_2 \mapsto 1,\ z_3 \mapsto \infty
  \]
  Similarly, we can write down a $\beta \in \mob$ such that:
  \[
    \beta: w_1 \mapsto 0,\ w_2 \mapsto 1,\ w_3 \mapsto \infty
  \]
  Thus we have:
  \[
    \beta^{-1} \circ \alpha: z_1 \mapsto w_1,\ z_2 \mapsto w_2,\ z_3 \mapsto w_3
  \]
  So $\mu = \beta^{-1} \circ \alpha$ works.
\end{proof}
\begin{remark}
  The above $\mu$ is unique as if we had some other $\nu \in \mob$ with
  \[
    \nu: z_1 \mapsto w_1,\ z_2 \mapsto w_2,\ z_3 \mapsto w_3
  \]
  then $\{z_1, z_2, z_3\} \subseteq \Fix(\nu^{-1} \circ \mu)$ so by \cref{threePointMob}, $\nu^{-1} \circ \mu = \id$ so $\nu = \mu$.

  We say that the action of $\mob$ on $\Cinf$ is \textit{sharply triple transitive}.
\end{remark}
\section{Cross Ratio}
\begin{definition}[Cross Ratio]
  Let $z_1, z_2, z_3, z_4 \in \Cinf$ be distinct.
  Because $\mob \acts \Cinf$ sharply triple transitively, there is a unique $\alpha \in \mob$ such that:
  \[
    \alpha(z_1) = 0,\ \alpha(z_2) = 1,\ \alpha(z_3) = \infty
  \]
  The \textit{cross-ratio} is then defined to be:
  \[
    [z_1, z_2, z_3, z_4] = \alpha(z_4)
  \]
\end{definition}
\begin{remark}[Note]
  We see from \cref{tripleTransitivity} that:
  \[
    [z_1, z_2, z_3, z_4] = \left(\frac{z_4 - z_1}{z_4 - z_3}\right)\left(\frac{z_2 - z_3}{z_2 - z_1}\right)
  \]
\end{remark}
\section{Generating Set}
Similarly to the Dihedral groups, we can use the three-point lemma to find a generating set for $\mob$.
\begin{proposition}
  $\mob$ is generated by the set of elements of the following three forms:
  \begin{enumerate}
    \item $\alpha_a : z \mapsto az,\ a \neq 0$
    \item $\beta_b: z \mapsto z + b,\ b \in \C$
    \item $\gamma: z \mapsto \frac{1}{z}$
  \end{enumerate}
\end{proposition}
\begin{remark}
  We should \textbf{not} claim that something is \textit{the} generating set, just that it is \textit{a} generating set of the group.
\end{remark}
\begin{proof}
  Let $\mu \in \mob$ be an arbitrary M\"obius transform, and let $z_1 = \mu(0), z_2 = \mu(1), z_3 = \mu(\infty)$.
  Note that since M\"obius transforms are invertible, $z_1$, $z_2$, and $z_3$ must be distinct.

  \textbf{Step 1 -}
  We first need to construct a $\mu_1$ such that $\mu_1(z_3) = \infty$.

  Either $z_3$ is already infinity so we can take $\mu_1 = \id$, otherwise let $b = -z_3$ and let:
  \[
    \mu_1(z) = \frac{1}{z+b} = \gamma \circ \beta_b
  \]
  To keep track of where this sends the other two points, let $z_1' = \mu_1(z_1)$ and $z_2' = \mu_1(z_2)$.
  Note that neither $z_1'$ or $z_2'$ can be infinity as the points are distinct.

  \textbf{Step 2 -}
  We now need to construct a $\mu_2$ such that $\mu_2(z_1') = 0$ and $\mu_2(\infty) = \infty$.

  Let $b' = - z_1'$ and let $\mu_2$:
  \[
    \mu_2(z) = z + b' = \beta_{b'}
  \]
  Therefore, $\mu_2(z_1') = 0,\ \mu_2(\infty) = \infty$.
  To keep track of where this sends, $z_2'$, let $z_2'' = \mu_2(z_2')$.
  Note that $z_2''$ cannot be infinity or 0.

  \textbf{Step 3 -}
  Finally, we need to construct a $\mu_3$ such that $\mu_3(z_2'') = 1$, $\mu_3(0) = 0$ and $\mu_3(\infty) = \infty$.

  Let $a = \frac{1}{z_2''}$ and let:
  \[
    \mu_3 (z) = az = \alpha_a
  \]
  Therefore, $\mu_3(z_2'') = 1,\ \mu_3(0) = 0,\ \mu_3(\infty) = \infty$.

  \textbf{Summary -}
  So by construction:
  \begin{align*}
    \mu_3 \circ \mu_2 \circ \mu_1 (z_1) &= \mu_3 \circ \mu_2 (z_1') = \mu_3(0) = 0 \\
    \mu_3 \circ \mu_2 \circ \mu_1 (z_2) &= \mu_3 \circ \mu_2 (z_2') = \mu_3(z_2'') = 1 \\
    \mu_3 \circ \mu_2 \circ \mu_1 (z_3) &= \mu_3 \circ \mu_2 (\infty) = \mu_3(\infty) = \infty
  \end{align*}
  We can now invert this so that $(\mu_3 \circ \mu_2 \circ \mu_1)^{-1} = \mu^{-1}_{1} \circ \mu^{-1}_{2} \circ \mu^{-1}_{3}$ sends:
  \[
    \mu^{-1}_{1} \circ \mu^{-1}_{2} \circ \mu^{-1}_{3}: 0 \mapsto z_1,\ 1 \mapsto z_2,\ \infty \mapsto z_3
  \]
  This is the same as $\mu$ on three distinct points, therefore by \cref{threePointMob}, $\mu = \mu^{-1}_{1} \circ \mu^{-1}_{2} \circ \mu^{-1}_{3}$ which is a combination of the three generators.
\end{proof}
\section{Circles}
\subsection{Generalised Circles}
\begin{definition}[Circle in $\Cinf$]
  A \textit{circle in} $\Cinf$ is either:
  \begin{enumerate}
    \item  A Euclidean circle in $\C$
    \item $l \cup \{\infty\}$ where $l \subseteq \C$ is a Euclidean straight line.
  \end{enumerate}
\end{definition}
Euclidean circles are defined by the equation:
\[
  |z - c| = r \quad z, c\in \C,\ r \in \R^{+}
\]
whilst lines are defined by:
\[
  |z - a| = |z - b| \quad z, a, b \in \C
\]
which is the perpendicular bisector of the line joining $a$ and $b$.
\subsection{Preserving Circles}
\begin{theorem}[Circles and M\"obius Transformations]
  If $C \subseteq \Cinf$ is a circle and $\mu \in \mob$, then $\mu(C)$ is also a circle.
\end{theorem}
\begin{proof}
  Recall that $\mob$ is generated by:
  \begin{itemize}
    \item $\alpha_a : z \mapsto az,\ a \neq 0$
    \item $\beta_b: z \mapsto z + b,\ b \in \C$
    \item $\gamma: z \mapsto \frac{1}{z}$
  \end{itemize}
  So it is sufficient to check that $\alpha_a(C)$, $\beta_b(C)$, and $\gamma(C)$ are all circles.
  For $\alpha_a$ and $\beta_b$, this is easy as dilations, rotations, and translations preserve euclidean circles and lines.
  So we just need to check it for $\gamma$.
  \begin{proofcases}
    \begin{case}{$C$ is a Euclidean Circle}
      If $C$ is a Euclidean circle, then $\gamma(C)$ has equation:
      \begin{align*}
        \abs{\frac{1}{z} - c} &= r \\
        \abs{\frac{1}{z} - c}^2 &= r^2 \\
        \left(\frac{1}{z} - c\right)\left(\frac{1}{z^{*}} - c^{*}\right) &= r^2 \\
        \frac{1}{|z|^2} - \frac{c}{z^{*}} - \frac{c^{*}}{z} + |c|^2 -r^2 &= 0 \\
        \left(|c|^2 - |r|^2\right)|z|^2 - cz - c^{*}z^{*} + 1 &= 0
      \end{align*}
      If $|c|^2 = |r|^2$, then the equation becomes:
      \begin{align*}
        cz + c^{*}z^{*} &= 1 \\
        \frac{z}{c^{*}} + \frac{z^{*}}{c} &= \frac{1}{|c|^2} \\
        |z|^2 &= |z|^2 - \frac{z}{c^{*}} - \frac{z^{*}}{c} + \frac{1}{|c|^2} \\
        |z|^2 &= \abs{z - \frac{1}{c}}^2 \\
        |z| &= \abs{z - \frac{1}{c}}
      \end{align*}
      which is a straight line, as required.

      Otherwise, if $|c|^2 \neq |r|^2$ then the equation becomes:
      \begin{align*}
        |z|^2 - \left(\frac{c}{|c|^2 - r^2}\right) z - \left(\frac{c^{*}}{|c|^2 - r^2}\right)z^{*} + \frac{1}{|c|^2 - r^2} &= 0 \\
        \abs{z - \frac{c^{*}}{|c|^2 - r^2}}^2 &= \frac{|c|^2}{(|c|^2 - r^2)^2} - \frac{1}{|c|^2 - r^2} \\
        \abs{z - \frac{c^{*}}{|c|^2 - r^2}}^2 &= \frac{r^2}{(|c|^2 - r^2)^2} \\
        \abs{z - \frac{c^{*}}{|c|^2 - r^2}} &= \frac{r}{\abs{|c|^2 - r^2}} \in \R^{+}
      \end{align*}
      which is a circle.
    \end{case}
    \begin{case}{$C$ is a line}
      If $C$ is a Euclidean line, then $\gamma(C)$ has equation:
      \begin{align*}
        \abs{\frac{1}{z} - a} &= \abs{\frac{1}{z} - b} \\
        \abs{\frac{1}{z} - a}^2 &= \abs{\frac{1}{z} - b}^2 \\
        \left(\frac{1}{z} - a\right)\left(\frac{1}{z^{*}} - a^{*}\right) &= \left(\frac{1}{z} - b\right)\left(\frac{1}{z^{*}} - b^{*}\right) \\
        \cancel{\frac{1}{z^2}} - \frac{a}{z^{*}} - \frac{a^{*}}{z} + |a|^2 &= \cancel{\frac{1}{z^2}} - \frac{b}{z^{*}} - \frac{b^{*}}{z} + |b|^2 \\
        |z|^2(|a|^2 - |b|^2) - z(a - b) - z^{*}(a^{*} - b^{*}) &= 0
      \end{align*}
      If $|a|^2 = |b|^2$, then the equation becomes:
      \begin{align*}
        z(a - b) + z^{*}(a^{*} - b^{*}) &= 0 \\
        \left(\frac{a}{2} - \frac{b}{2}\right)z - \left(\frac{b}{2} - \frac{a}{2}\right)z &+ \left(\frac{a^{*}}{2} - \frac{b^{*}}{2}\right)z^{*} - \left(\frac{b^{*}}{2} - \frac{a^{*}}{2}\right)z^{*} = 0 \\
        -\left(\frac{b}{2} - \frac{a}{2}\right)z - \left(\frac{b^{*}}{2} - \frac{a^{*}}{2}\right)z^{*} &= -\left(\frac{a}{2} - \frac{b}{2}\right)z -\left(\frac{a^{*}}{2} - \frac{b^{*}}{2}\right)z^{*}
      \end{align*}
      We can then add $|z|^2$ and $\frac{|a - b|^2}{4}$ to both sides to yield:
      \[
        \abs{z - \frac{b^{*} - a^{*}}{2}} = \abs{z - \frac{a^{*} - b^{*}}{2}}
      \]
      which is a straight line.

      Otherwise, if $|a|^2 \neq |b|^2$ then the equation becomes:
      \begin{align*}
        |z|^2(|a|^2 - |b|^2) - z(a - b) - z^{*}(a^{*} - b^{*}) &= 0 \\
        |z|^2 - \left(\frac{a - b}{|a|^2 - |b|^2}\right)z - \left(\frac{a^{*} - b^{*}}{|a|^2 - |b|^2}\right)z^{*} &= 0 \\
        |z|^2 - \left(\frac{a - b}{|a|^2 - |b|^2}\right)z - \left(\frac{a^{*} - b^{*}}{|a|^2 - |b|^2}\right)z^{*} + \frac{|a - b|^2}{(|a|^2 - |b|^2)^2} &= \frac{|a - b|^2}{(|a|^2 - |b|^2)^2} \\
        \abs{z - \frac{a^{*} - b^{*}}{|a|^2 - |b|^2}}^2 &= \frac{|a -  b|^2}{(|a|^2 - |b|^2)^2} \\
        \abs{z - \frac{a^{*} - b^{*}}{|a|^2 - |b|^2}} &= \frac{|a -  b|}{\abs{|a|^2 - |b|^2}} \in \R^{+}\\
      \end{align*}
      which is a circle.
    \end{case}
  \end{proofcases}
  In all cases, $\gamma$ sends generalised circles to generalised circles.
\end{proof}
\begin{corollary}
  Four points $z_1, z_2, z_3, z_4 \in \Cinf$ lie on a circle if and only if:
  \[
    [z_1, z_2, z_3, z_4] \in \R \cup \{\infty\}
  \]
\end{corollary}
\begin{proof}
  Let $\alpha \in \mob$ such that:
  \[
    \alpha(z_1) = 0,\ \alpha(z_2) = 1,\ \alpha(z_3) = \infty
  \]
  so $[z_1, z_2, z_3, z_4] = \alpha(z_4)$ by definition.
  \begin{proofdirection}{Assume the points lie on a circle}
    If $z_1, z_2, z_3, z_4$ lie on a circle, then $0, 1, \infty, \alpha(z_4)$ will lie on $\alpha(C)$, which, by the theorem is also a circle.
    But the only circle containing $0, 1, \infty$ is the line $\R \cup \{\infty\}$ so $\alpha(z_4) \in \R \cup \{\infty\}$.
  \end{proofdirection}
  \begin{proofdirection}{Assume $\alpha(z_4) \in \R \cup \{\infty\}$}
    If $\alpha(z_4) \in \R \cup \{\infty\}$, which we know is a circle that $0, 1, \infty$ lie on.
    Therefore:
    \[
      z_1, \ldots, z_4 \in \alpha^{-1} (\R \cup \{\infty\})
    \]
    which is also a circle by the theorem.
  \end{proofdirection}
\end{proof}
\end{document}
